add ICom.deleteVar? Now use it to implement full DCE

SSA/Core/ErasedContext.lean
@@ -210,8 +210,37 @@ def Valuation.snoc {Γ : Ctxt Ty} {t : Ty} (s : Γ.Valuation) (x : toType t) :
   intro t' v
   revert s x
   refine Ctxt.Var.casesOn v ?_ ?_
-  . intro _ _ _ v s _; exact s v
+  . intro _ _ _ v s _;  exact s v
   . intro _ _ _ x; exact x
+
+def Valuation.snoc' {Γ : Ctxt Ty} {t : Ty} (s : Γ.Valuation) (x : toType t) : 
+    (Γ.snoc t).Valuation := 
+    fun t' var =>
+    match var with
+    | ⟨i, hvar⟩ =>  
+      match i with
+      | 0 => by
+        simp[Ctxt.snoc] at hvar
+        exact (hvar ▸ x)
+      | .succ i' => s ⟨i', hvar⟩
+
+/-- Show the equivalence between the definition in terms of `snoc` and `snoc'`. -/
+theorem Valuation.snoc_eq_snoc' {Γ : Ctxt Ty} {t : Ty} (s : Γ.Valuation) (x : toType t) 
+  : (s.snoc x) = (s.snoc' x):= by
+    simp[snoc, snoc']
+    funext t' v
+    cases V:v
+    case mk i hi => 
+      simp
+      simp[Var.casesOn]
+      cases i
+      case zero => 
+        simp
+        simp[Ctxt.snoc] at hi
+        subst hi
+        simp
+      case succ i' => 
+        simp
 
 @[simp]
 theorem Valuation.snoc_last {Γ : Ctxt Ty} {t : Ty} (s : Γ.Valuation) (x : toType t) :
